Cvc/Tmp.lean
@@ -1,0 +1,15 @@
+module
+
+import Cvc.Untyped
+meta import Cvc.Untyped
+
+
+namespace Cvc.Untyped
+
+
+
+#eval Env.runIO do
+  let int ← Srt.int
+  let bool ← Srt.bool
+  let record ← Srt.record #[("intField", int), ("boolField", bool)]
+  println! "record : {record}\n- is datatype := {record.isDatatype}"
