Cvc/Types/Tuple.lean
@@ -28,8 +28,8 @@ abbrev isFlat : Typ → Bool
   | prod _ => false
   | bool | int | real | string | regex | roundingMode
   | bitVec _ | float _ _ | finiteField _ | arrayTo _ _
-  | bag _ | set _ | seq _ | nullable _
-  | datatype _ | abstract _ | function _ _ | uninterpreted _ => true
+  | bag _ | set _ | seq _ | nullable _ | record _
+  | datatype _ | function _ _ | uninterpreted _ => true
 
 end Typ
 
